fix the (VAR) rule

Capless/Typing.lean
@@ -83,10 +83,8 @@ inductive Captured : Term n m k -> CaptureSet n k -> Prop where
 
 inductive Typed : Context n m k -> Term n m k -> EType n m k -> Prop where
 | var :
-  Context.Bound Γ x T ->
-  /- TODO Apparently I made a mistake here, fix it afterwards
-   -   so that it will not disturb the on-going proof -/
-  Typed Γ (Term.var x) (EType.type T)
+  Context.Bound Γ x (CType.capt C S) ->
+  Typed Γ (Term.var x) (EType.type (CType.capt {x} S))
 | pack :
   Typed (Γ.cvar (CBinding.inst C)) (Term.var x) (EType.type T) ->
   Typed Γ (Term.pack C x) (EType.ex T)
